Memory compartments in Asm
The most interesting question is: where should we expose the existence
of compartments in the execution of Asm instructions? Unlike at other
levels the answer is not completely straightforward.

A possibility is to encapsulate these accesses inside [exec_instr],
essentially wrapping the original definition with checks to retrieve the
necessary (and readily available) information from the environment,
namely the PC component and its associated component. This choice
appears to be more self-contained, but certain results that require us
to establish, say, the successful execution of an instruction may
require additional assumptions (i.e., that the PC always contains a
pointer value and that its component lookup always succeeds).
Additionally, proofs on the wrapped version of [exec_instr] may have to
perform extra work to expose its underlying native form.

The other main possibility is to parameterize [exec_instr] on a
compartment and supply this information externally as needed. This
option requires a larger number of (minor) changes, but no additional
information. However, although the added compartment in [exec_instr]
needs to be added to all theorems using this definition, this parameter
is only of use for loads and stores, and unspecified in other cases. For
this reason, main helper lemmas, in particular [exec_straight_one], need
to be applied existentially, yet at the end their compartment variable
remains uninstantiated. Some local invariants need to be strengthened,
also straightforwardly, with compartment equality on memory operations.

backend/Asmgenproof0.v
@@ -358,7 +358,7 @@ Proof.
   exploit Mem.loadv_extends; eauto. intros [v' [A B]].
   rewrite (sp_val _ _ _ H) in A.
   exists v'; split; auto.
-  econstructor. eauto. assumption.
+  econstructor. eauto. eassumption.
 Qed.
 
 Lemma extcall_arg_pair_match:
@@ -804,13 +804,13 @@ Variable fn: function.
 Inductive exec_straight: code -> regset -> mem ->
                          code -> regset -> mem -> Prop :=
   | exec_straight_one:
-      forall i1 c rs1 m1 rs2 m2,
-      exec_instr ge fn i1 rs1 m1 = Next rs2 m2 ->
+      forall i1 c rs1 m1 cp rs2 m2,
+      exec_instr ge fn i1 rs1 m1 cp = Next rs2 m2 ->
       rs2#PC = Val.offset_ptr rs1#PC Ptrofs.one ->
       exec_straight (i1 :: c) rs1 m1 c rs2 m2
   | exec_straight_step:
-      forall i c rs1 m1 rs2 m2 c' rs3 m3,
-      exec_instr ge fn i rs1 m1 = Next rs2 m2 ->
+      forall i c rs1 m1 cp rs2 m2 c' rs3 m3,
+      exec_instr ge fn i rs1 m1 cp = Next rs2 m2 ->
       rs2#PC = Val.offset_ptr rs1#PC Ptrofs.one ->
       exec_straight c rs2 m2 c' rs3 m3 ->
       exec_straight (i :: c) rs1 m1 c' rs3 m3.
@@ -822,33 +822,33 @@ Lemma exec_straight_trans:
   exec_straight c1 rs1 m1 c3 rs3 m3.
 Proof.
   induction 1; intros.
-  apply exec_straight_step with rs2 m2; auto.
-  apply exec_straight_step with rs2 m2; auto.
+  apply exec_straight_step with cp0 rs2 m2; auto.
+  apply exec_straight_step with cp0 rs2 m2; auto.
 Qed.
 
 Lemma exec_straight_two:
-  forall i1 i2 c rs1 m1 rs2 m2 rs3 m3,
-  exec_instr ge fn i1 rs1 m1 = Next rs2 m2 ->
-  exec_instr ge fn i2 rs2 m2 = Next rs3 m3 ->
+  forall i1 i2 c rs1 m1 cp1 rs2 m2 cp2 rs3 m3,
+  exec_instr ge fn i1 rs1 m1 cp1 = Next rs2 m2 ->
+  exec_instr ge fn i2 rs2 m2 cp2 = Next rs3 m3 ->
   rs2#PC = Val.offset_ptr rs1#PC Ptrofs.one ->
   rs3#PC = Val.offset_ptr rs2#PC Ptrofs.one ->
   exec_straight (i1 :: i2 :: c) rs1 m1 c rs3 m3.
 Proof.
-  intros. apply exec_straight_step with rs2 m2; auto.
-  apply exec_straight_one; auto.
+  intros. apply exec_straight_step with cp1 rs2 m2; auto.
+  eapply exec_straight_one; eauto.
 Qed.
 
 Lemma exec_straight_three:
-  forall i1 i2 i3 c rs1 m1 rs2 m2 rs3 m3 rs4 m4,
-  exec_instr ge fn i1 rs1 m1 = Next rs2 m2 ->
-  exec_instr ge fn i2 rs2 m2 = Next rs3 m3 ->
-  exec_instr ge fn i3 rs3 m3 = Next rs4 m4 ->
+  forall i1 i2 i3 c rs1 m1 cp1 rs2 m2 cp2 rs3 m3 cp3 rs4 m4,
+  exec_instr ge fn i1 rs1 m1 cp1 = Next rs2 m2 ->
+  exec_instr ge fn i2 rs2 m2 cp2 = Next rs3 m3 ->
+  exec_instr ge fn i3 rs3 m3 cp3 = Next rs4 m4 ->
   rs2#PC = Val.offset_ptr rs1#PC Ptrofs.one ->
   rs3#PC = Val.offset_ptr rs2#PC Ptrofs.one ->
   rs4#PC = Val.offset_ptr rs3#PC Ptrofs.one ->
   exec_straight (i1 :: i2 :: i3 :: c) rs1 m1 c rs4 m4.
 Proof.
-  intros. apply exec_straight_step with rs2 m2; auto.
+  intros. apply exec_straight_step with cp1 rs2 m2; auto.
   eapply exec_straight_two; eauto.
 Qed.
 
@@ -932,20 +932,20 @@ Proof.
 Qed.
 
 Lemma exec_straight_opt_step:
-  forall i c rs1 m1 rs2 m2 c' rs3 m3,
-  exec_instr ge fn i rs1 m1 = Next rs2 m2 ->
+  forall i c rs1 m1 cp rs2 m2 c' rs3 m3,
+  exec_instr ge fn i rs1 m1 cp = Next rs2 m2 ->
   rs2#PC = Val.offset_ptr rs1#PC Ptrofs.one ->
   exec_straight_opt c rs2 m2 c' rs3 m3 ->
   exec_straight (i :: c) rs1 m1 c' rs3 m3.
 Proof.
   intros. inv H1. 
-- apply exec_straight_one; auto.
+- eapply exec_straight_one; eauto.
 - eapply exec_straight_step; eauto.
 Qed.
 
 Lemma exec_straight_opt_step_opt:
-  forall i c rs1 m1 rs2 m2 c' rs3 m3,
-  exec_instr ge fn i rs1 m1 = Next rs2 m2 ->
+  forall i c rs1 m1 cp rs2 m2 c' rs3 m3,
+  exec_instr ge fn i rs1 m1 cp = Next rs2 m2 ->
   rs2#PC = Val.offset_ptr rs1#PC Ptrofs.one ->
   exec_straight_opt c rs2 m2 c' rs3 m3 ->
   exec_straight_opt (i :: c) rs1 m1 c' rs3 m3.
